nbe.v
@@ -1,4 +1,5 @@
 From WR Require Export syntax.
+From Hammer Require Import Tactics.
 
 Inductive Domain : Type :=
 | D_Abs : tm -> (nat -> Domain) -> Domain
@@ -24,9 +25,9 @@ with DEval : Env -> tm -> Domain -> Prop :=
   (* ------------------------ *)
   DEval ρ (var_tm i) (ρ i)
 
-| DE_Abs ρ A a :
+| DE_Abs ρ a :
   (* --------------------------- *)
-  DEval ρ (Lam A a) (D_Abs a ρ)
+  DEval ρ (Lam a) (D_Abs a ρ)
 
 | DE_App ρ a f b d d0 :
   DEval ρ a f ->
@@ -34,3 +35,33 @@ with DEval : Env -> tm -> Domain -> Prop :=
   DApp f d d0 ->
   (* -------------------- *)
   DEval ρ (App a b) d0.
+
+
+Inductive RB n : Domain -> tm -> Prop :=
+| B_AppAbs ρ b t t0  :
+  DEval (D_Ne (N_Var n) .: ρ) t b ->
+  RB (S n) b t0 ->
+  RB n (D_Abs t ρ) (Lam t0)
+| B_Ne e t :
+  RBNe n e t ->
+  RB n (D_Ne e) t
+with RBNe n : DomainNe -> tm -> Prop :=
+| B_Var i :
+  RBNe n (N_Var i) (var_tm (n - (S i)))
+| B_App e f t0 t1 :
+  RBNe n e t0 ->
+  RB n f t1 ->
+  RBNe n (D_App e f) (App t0 t1).
+
+Definition init_env n : Env := fun i => D_Ne (N_Var (n - (S i))).
+
+Definition norm n a b := exists d, DEval (init_env n) a d /\ RB n d b.
+
+Example test0 : norm 0 (App (Lam (var_tm 0)) (Lam (var_tm 0))) (Lam (var_tm 0)).
+Proof. sauto lq:on rew:off. Qed.
+
+Example test1 : norm 1 (App (Lam (var_tm 0)) (var_tm 0)) (var_tm 0).
+Proof. sauto lq:on rew:off. Qed.
+
+Example test2 : norm 1 (App (Lam (App (var_tm 0) (var_tm 1))) (var_tm 0)) (App (var_tm 0) (var_tm 0)).
+Proof. sauto lq:on rew:off. Qed.
