typing.v
@@ -12,7 +12,7 @@ Inductive Wt (n : nat) (Γ : context) : tm -> ty -> Prop :=
 | T_Lam : forall A a B,
     Wt (S n) (A .: Γ) a B ->
     (* -------------------------- *)
-    Wt n Γ (Lam A a) (Fun A B)
+    Wt n Γ (Lam a) (Fun A B)
 
 | T_App : forall a A B b,
     Wt n Γ a (Fun A B) ->
